Fixup LLM output.

code/bignum/Hacl.Bignum.LibPulse.fst
@@ -8,10 +8,12 @@ open Hacl.Bignum.BasePulse
 open Hacl.Bignum.DefinitionsPulse
 
 module S = Hacl.Spec.Bignum.Lib
+module SD = Hacl.Spec.Bignum.Definitions
 module SL = Hacl.Spec.Lib
 module LSeq = Lib.Sequence
 module AP = Pulse.Lib.ArrayPtr
 module AR = Lib.ArrayRefPulse
+module Loops = Lib.LoopCombinators
 
 inline_for_extraction let sizet_of_size_t (x: size_t) : y:SizeT.t { v x == SizeT.v y } =
   assume SizeT.fits_u32;
@@ -27,16 +29,17 @@ fn bn_get_ith_bit
   (len:size_t)
   (b:lbignum t len)
   (i:size_t{v i / bits t < v len})
-  requires pts_to b (b0)
+  (#b0: erased (SD.lbignum t (v len))) #prb
+  requires pts_to b #prb b0
   returns r:limb t
-  ensures pts_to b (b0)
+  ensures pts_to b #prb b0
   ensures pure (r == S.bn_get_ith_bit (b0) (v i))
 {
   let pbits = size (bits t);
   let i_ind = i /. pbits;
   let j = i %. pbits;
   let tmp = AP.(b.(sizet_of_size_t i_ind));
-  (tmp >>. j) &. (uint #t 1)
+  ((tmp >>. j) &. (uint #t 1))
 }
 
 inline_for_extraction noextract
@@ -45,14 +48,16 @@ fn bn_set_ith_bit
   (len:size_t)
   (b:lbignum t len)
   (i:size_t{v i / bits t < v len})
+  (#b0: erased (SD.lbignum t (v len)))
   requires pts_to b (b0)
-  returns ()
   ensures pts_to b (S.bn_set_ith_bit (b0) (v i))
 {
   let pbits = size (bits t);
   let i_ind = i /. pbits;
+  assert pure (v i_ind < v len); // Z3 fails nondeterministically without this
   let j = i %. pbits;
-  AP.(b.(sizet_of_size_t i_ind)) <- AP.(b.(sizet_of_size_t i_ind)) |. (uint #t 1 <<. j)
+  let b_i_ind = AP.(b.(sizet_of_size_t i_ind));
+  AP.(b.(sizet_of_size_t i_ind) <- b_i_ind |. (uint #t 1 <<. j));
 }
 
 inline_for_extraction noextract
@@ -62,43 +67,78 @@ fn cswap2_st
   (bit:limb t)
   (b1:lbignum t len)
   (b2:lbignum t len)
+  (#b1_0: erased (SD.lbignum t (v len)))
+  (#b2_0: erased (SD.lbignum t (v len)))
   requires pts_to b1 (b1_0) ** pts_to b2 (b2_0)
-  returns ()
   ensures pts_to b1 (fst (S.cswap2 bit b1_0 b2_0)) ** pts_to b2 (snd (S.cswap2 bit b1_0 b2_0))
 {
   let mask = (uint #t 0) -. bit;
   let mut i = 0ul;
-  let len_sizet = sizet_of_size_t len;
-  let body_ty = 
-    fun i x1 x2 -> pts_to b1 x1 ** pts_to b2 x2;
-  let body () = i #x1 #x2 {
-    let dummy = mask &. (AP.(b1.(sizet_of_size_t i)) ^. AP.(b2.(sizet_of_size_t i)));
-    AP.(b1.(sizet_of_size_t i)) <- AP.(b1.(sizet_of_size_t i)) ^. dummy;
-    AP.(b2.(sizet_of_size_t i)) <- AP.(b2.(sizet_of_size_t i)) ^. dummy;
+  Loops.eq_repeati0 0 (S.cswap2_f mask) (reveal b1_0, reveal b2_0);
+  while (let vi = !i; lt vi len)
+    invariant b. exists* vi vb1 vb2.
+      pts_to b1 vb1 ** pts_to b2 vb2 ** pts_to i vi **
+      pure (b == lt vi len) **
+      pure (v vi <= v len /\
+        (vb1, vb2) == Loops.repeati (v vi) (S.cswap2_f mask) (reveal b1_0, reveal b2_0))
+  {
+    let vi = !i;
+    let b1_i = AP.(b1.(sizet_of_size_t vi));
+    let b2_i = AP.(b2.(sizet_of_size_t vi));
+    let dummy = mask &. (b1_i ^. b2_i);
+    AP.(b1.(sizet_of_size_t vi) <- b1_i ^. dummy);
+    AP.(b2.(sizet_of_size_t vi) <- b2_i ^. dummy);
+    Loops.unfold_repeati (v len) (S.cswap2_f mask) (reveal b1_0, reveal b2_0) (v vi);
+    i := add vi 1ul;
   };
-  fill_elems4 body_ty len_sizet (body ());
 }
 
 inline_for_extraction noextract
-fn bn_get_top_index
-  (#t:limb_t)
-  (len:size_t{0 < v len})
-  (b:lbignum t len)
-  requires pts_to b (b0)
-  returns r:limb t
-  ensures pts_to b (b0)
-  ensures pure (r == S.bn_get_top_index (b0))
-{
-  let mut r = 0ul;
-  let len_sizet = sizet_of_size_t len;
-  let body_ty = fun i x0 -> pts_to b x0;
-  let body () = i #x0 {
-    let mask = eq_mask (AP.(b.(sizet_of_size_t i))) (zeros t SEC);
-    r <- mask_select mask r (size_to_limb i);
+let bn_get_top_index_st (t:limb_t) (len:size_t{0 < v len}) =
+  b:lbignum t len -> #b0: erased (SD.lbignum t (v len)) -> #prb: perm ->
+  stt (limb t) (requires pts_to b #prb b0)
+    fun r -> pts_to b #prb b0 **
+      pure (v r == S.bn_get_top_index b0)
+
+inline_for_extraction noextract
+fn mk_bn_get_top_index (#t: limb_t) (len: size_t { 0 < v len }) :
+    bn_get_top_index_st t len = b #b0 #prb {
+  let mut r = (uint 0 <: limb t);
+  with vr0. assert pts_to r vr0;
+
+  with spec. assert pure (spec == S.bn_get_top_index_f b0);
+  Loops.eq_repeat_gen0 (v len) (S.bn_get_top_index_t (v len)) spec (v vr0);
+  let mut i = 0ul;
+  while (let vi = !i; lt vi len)
+    invariant cond. exists* vi vr.
+      pts_to i vi ** pts_to r vr ** pts_to b #prb b0 **
+      pure (cond == lt vi len) **
+      pure (v vi <= v len /\
+        v vr == Loops.repeat_gen (v vi) (S.bn_get_top_index_t (v len)) spec (v vr0))
+  {
+    let vi = !i;
+    Loops.unfold_repeat_gen (v len) (S.bn_get_top_index_t (v len)) spec (v vr0) (v vi);
+    let b_i = AP.(b.(sizet_of_size_t vi));
+    let mask = eq_mask b_i (zeros t SEC);
+    let vr = !r;
+    r := mask_select mask vr (size_to_limb vi);
+    mask_select_lemma mask vr (size_to_limb vi);
+    i := add vi 1ul;
   };
-  fill_elems4 body_ty len_sizet (body ());
-  r
+
+  !r
 }
+
+let bn_get_top_index_u32 len: bn_get_top_index_st U32 len = mk_bn_get_top_index #U32 len
+let bn_get_top_index_u64 len: bn_get_top_index_st U64 len = mk_bn_get_top_index #U64 len
+
+
+inline_for_extraction noextract
+val bn_get_top_index: #t:_ -> len:_ -> bn_get_top_index_st t len
+let bn_get_top_index #t =
+  match t with
+  | U32 -> bn_get_top_index_u32
+  | U64 -> bn_get_top_index_u64
 
 
 inline_for_extraction noextract
@@ -107,17 +147,20 @@ fn bn_get_bits_limb
   (len:size_t)
   (b:lbignum t len)
   (i:size_t{v i / bits t < v len})
-  requires pts_to b (b0)
+  (#b0: erased (SD.lbignum t (v len))) #prb
+  requires pts_to b #prb b0
   returns r:limb t
-  ensures pts_to b (b0)
+  ensures pts_to b #prb b0
   ensures pure (r == S.bn_get_bits_limb (b0) (v i))
 {
   let pbits = size (bits t);
   let i_ind = i /. pbits;
   let j = i %. pbits;
-  let p1 = AP.(b.(sizet_of_size_t i_ind)) >>. j;
+  let b_i_ind = AP.(b.(sizet_of_size_t i_ind));
+  let p1 = b_i_ind >>. j;
   if (i_ind +! 1ul <. len && 0ul <. j) {
-    p1 |. (AP.(b.(sizet_of_size_t (i_ind +! 1ul))) <<. (pbits -! j))
+    let b_ind_1 = AP.(b.(sizet_of_size_t (i_ind +! 1ul)));
+    (p1 |. (b_ind_1 <<. (pbits -! j)))
   } else {
     p1
   }
@@ -130,11 +173,13 @@ fn bn_get_bits
   (b:lbignum t len)
   (i:size_t)
   (l:size_t{v l < bits t /\ v i / bits t < v len})
-  requires pts_to b (b0)
+  (#b0: erased (SD.lbignum t (v len))) #prb
+  requires pts_to b #prb b0
   returns r:limb t
-  ensures pts_to b (b0)
+  ensures pts_to b #prb b0
   ensures pure (r == S.bn_get_bits (b0) (v i) (v l))
 {
-  let mask_l = (uint #t 1 <<. l) -. (uint #t 1);
-  bn_get_bits_limb len b i &. mask_l
+  let mask_l: limb t = (uint #t 1 <<. l) -. (uint #t 1);
+  let r = bn_get_bits_limb len b i;
+  (r &. mask_l)
 }
